theories/stacked_borrows/examples/opt2_down.v
@@ -6,8 +6,7 @@ From iris.prelude Require Import options.
 (** Moving a read of a shared reference down across code that *may* use that ref. *)
 
 (* Assuming x : & i32 *)
-Definition ex2_down_unopt : ectx :=
-  λ: "i",
+Definition ex2_down_unopt : expr :=
     let: "c" := InitCall in
     (* "x" is the local variable that stores the pointer value "i" *)
     let: "x" := new_place (& int) "i" in
@@ -32,8 +31,7 @@ Definition ex2_down_unopt : ectx :=
     "v"
   .
 
-Definition ex2_down_opt : ectx :=
-  λ: "i",
+Definition ex2_down_opt : expr :=
     let: "c" := InitCall in
     let: "x" := new_place (& int) "i" in
     retag_place "x" (RefPtr Immutable) int FnEntry "c";;
@@ -47,10 +45,11 @@ Definition ex2_down_opt : ectx :=
     "v"
   .
 
-Lemma sim_opt2_down `{sborGS Σ} π :
-  ⊢ sim_ectx π ex2_down_opt ex2_down_unopt rrel.
+Lemma sim_opt2_down `{sborGS Σ} :
+  ⊢ log_rel ex2_down_opt ex2_down_unopt.
 Proof.
-  iIntros (r_t r_s) "Hrel".
+  log_rel.
+  iIntros "%r_t %r_s #Hrel !# %π _".
   sim_pures.
   sim_apply InitCall InitCall sim_init_call "". iIntros (c) "Hcall". iApply sim_expr_base. sim_pures.
   sim_apply (Alloc _) (Alloc _) sim_alloc_local "". iIntros (t l) "Htag Ht Hs".
@@ -117,7 +116,8 @@ Proof.
     apply map_eq. intros t'. rewrite delete_insert_delete delete_insert; done.
   }
   sim_pures.
-  sim_val. iModIntro. destruct Hv_s' as [-> | ->]; first done.
+  sim_val. iModIntro. iSplit; first done.
+  destruct Hv_s' as [-> | ->]; first done.
   iApply big_sepL2_forall. iSplit. { rewrite replicate_length. iPureIntro. lia. }
   iIntros (k sc_t sc_s). rewrite lookup_replicate. iIntros "Hsc (-> & _)". destruct sc_t;done.
 Qed.
