theories/stacked_borrows/steps_retag.v
@@ -1,8 +1,6 @@
 From simuliris.stacked_borrows Require Export defs steps_foreach steps_list steps_wf steps_progress.
 From iris.prelude Require Import options.
 
-
-
 Definition tag_on_top (stks: stacks) l t pm : Prop :=
   ∃ prot, (stks !! l) ≫= head = Some (mkItem pm (Tagged t) prot).
 
